Start fixing slice proofs

new/golang/theory/slice.v
@@ -12,44 +12,50 @@ Set Default Proof Using "Type".
 Transparent slice.for_range slice.literal.
 
 Module slice.
-Definition slice_f (sl : slice.t) (t : go.type) (n1 n2 : u64) : slice.t :=
-  slice.mk (sl.(slice.ptr_f) +ₗ[t] sint.Z n1) (word.sub n2 n1) (word.sub sl.(slice.cap_f) n1).
+Section def.
+Context `{GoContext}.
+Definition slice (sl : slice.t) (et : go.type) (n1 n2 : u64) : slice.t :=
+  slice.mk (slice_index_ref et (sint.Z n1) sl) (word.sub n2 n1) (word.sub sl.(slice.cap) n1).
 
-Definition full_slice_f (sl : slice.t) (t : go_type) (n1 n2 n3 : u64) : slice.t :=
-  slice.mk (sl.(slice.ptr_f) +ₗ[t] sint.Z n1) (word.sub n2 n1) (word.sub n3 n1).
+Definition full_slice (sl : slice.t) (et : go.type) (n1 n2 n3 : u64) : slice.t :=
+  slice.mk (slice_index_ref et (sint.Z n1) sl) (word.sub n2 n1) (word.sub n3 n1).
+End def.
 End slice.
 
 Section defns_and_lemmas.
-Context `{ffi_syntax} `{ffi_interp}.
-Context `{!heapGS Σ}.
+Context `{ffi_sem: ffi_semantics} `{!ffi_interp ffi} `{!heapGS Σ}.
 
-Definition own_slice_def `{!IntoVal V} `{!IntoValTyped V t} (s : slice.t) (dq : dfrac) (vs : list V): iProp Σ :=
-  ([∗ list] i ↦ v ∈ vs, (s.(slice.ptr_f) +ₗ[t] i) ↦{dq} v ) ∗
-  ⌜length vs = sint.nat s.(slice.len_f) ∧ 0 ≤ sint.Z s.(slice.len_f) ≤ sint.Z s.(slice.cap_f)⌝.
+Definition own_slice_def {V} t `{!IntoVal V} `{!TypedPointsto V} `{!IntoValTyped V t}
+  (s : slice.t) (dq : dfrac) vs
+  : iProp Σ :=
+  ([∗ list] i ↦ v ∈ vs, (slice_index_ref t i s) ↦{dq} v ) ∗
+  ⌜ length vs = sint.nat s.(slice.len) ∧ 0 ≤ sint.Z s.(slice.len) ≤ sint.Z s.(slice.cap) ⌝.
 Program Definition own_slice := sealed @own_slice_def.
 Definition own_slice_unseal : own_slice = _ := seal_eq _.
 
-Global Arguments own_slice {_ _ _ _} (s dq vs).
+Global Arguments own_slice {_} (t) {_ _ _} (s dq vs).
 
-Notation "s ↦* dq vs" := (own_slice s dq vs)
-                            (at level 20, dq custom dfrac at level 50, format "s  ↦* dq  vs").
+Notation "s ↦[ t ]* dq vs" := (own_slice t s dq vs)
+                            (at level 20, dq custom dfrac at level 50, format "s  ↦[ t ]* dq  vs").
 
 Context `{!IntoVal V}.
+Context `{!TypedPointsto (Σ:=Σ) V}.
 Context `{!IntoValTyped V t}.
 Implicit Type (vs : list V).
+
 Definition own_slice_cap_def (s : slice.t) (dq : dfrac) : iProp Σ :=
-  ⌜ 0 ≤ sint.Z s.(slice.len_f) ≤ sint.Z s.(slice.cap_f) ⌝ ∗
+  ⌜ 0 ≤ sint.Z s.(slice.len) ≤ sint.Z s.(slice.cap) ⌝ ∗
 (* Two notes about this definition. First, it is written using [own_slice] to
 get some reuse, though an intermediate array points-to would be more useful
 here. Second, the capacity has arbitrary values, which is often desirable,
 but there are some niche cases where code could be aware of the contents of the
 capacity (for example, when sub-slicing from a larger slice) - actually taking
 advantage of that seems questionable though. *)
-  ∃ (vs: list V), own_slice
+  ∃ (vs: list V), own_slice t
                     (slice.mk
-                       (s.(slice.ptr_f) +ₗ[t] sint.Z s.(slice.len_f))
-                       (word.sub s.(slice.cap_f) s.(slice.len_f))
-                       (word.sub s.(slice.cap_f) s.(slice.len_f))) dq vs.
+                       (slice_index_ref t (sint.Z s.(slice.len)) s)
+                       (word.sub s.(slice.cap) s.(slice.len))
+                       (word.sub s.(slice.cap) s.(slice.len))) dq vs.
 Program Definition own_slice_cap := sealed @own_slice_cap_def.
 Definition own_slice_cap_unseal : own_slice_cap = _ := seal_eq _.
 
@@ -57,14 +63,14 @@ Ltac unseal := rewrite ?own_slice_unseal /own_slice_def
                  ?own_slice_cap_unseal /own_slice_cap_def.
 
 Lemma own_slice_nil dq :
-  ⊢ slice.nil ↦*{dq} ([] : list V).
+  ⊢ slice.nil ↦[t]*{dq} ([] : list V).
 Proof.
   unseal. simpl. iPureIntro. split_and!; done.
 Qed.
 
 Lemma own_slice_empty dq s :
-  sint.Z s.(slice.len_f) = 0 ->
-  0 ≤ sint.Z s.(slice.cap_f) ->
+  sint.Z s.(slice.len) = 0 ->
+  0 ≤ sint.Z s.(slice.cap) ->
   ⊢ s ↦*{dq} ([] : list V).
 Proof.
   unseal. intros Hsz Hcap. destruct s. simpl in *.
@@ -72,8 +78,8 @@ Proof.
 Qed.
 
 Lemma own_slice_cap_none s :
-  s.(slice.len_f) = s.(slice.cap_f) →
-  0 ≤ sint.Z s.(slice.len_f) →
+  s.(slice.len) = s.(slice.cap) →
+  0 ≤ sint.Z s.(slice.len) →
   ⊢ own_slice_cap s (DfracOwn 1).
 Proof.
   destruct s; simpl; intros -> Hlen. rewrite own_slice_cap_unseal /own_slice_cap_def /=.
@@ -85,7 +91,7 @@ Proof.
 Qed.
 
 Lemma own_slice_len s dq vs :
-  s ↦*{dq} vs -∗ ⌜length vs = sint.nat s.(slice.len_f) ∧ 0 ≤ sint.Z s.(slice.len_f)⌝.
+  s ↦*{dq} vs -∗ ⌜length vs = sint.nat s.(slice.len) ∧ 0 ≤ sint.Z s.(slice.len)⌝.
 Proof.
   unseal. iIntros "(_&[%%]) !%"; word.
 Qed.
@@ -106,7 +112,7 @@ Proof.
   unseal.
   iIntros "[Hs1 [%%]] [Hs2 [%%]]".
   assert (length vs1 = length vs2) by congruence.
-  generalize (slice.ptr_f s). intros l.
+  generalize (slice.ptr s). intros l.
   assert (length vs1 = length vs2) as Hlen by done.
   clear -Hlen IntoValTyped0.
   (iInduction vs1 as [|v1 vs1] "IH" forall (l vs2 Hlen)).
@@ -220,7 +226,7 @@ Lemma own_slice_not_null s dq vs :
   go_type_size t > 0 →
   length vs > 0 ->
   s ↦*{dq} vs -∗
-  ⌜ s.(slice.ptr_f) ≠ null ⌝.
+  ⌜ s.(slice.ptr) ≠ null ⌝.
 Proof using Type*.
   unseal.
   iIntros (Hbt Hvs) "[Hs %]".
@@ -232,7 +238,7 @@ Proof using Type*.
 Qed.
 
 Lemma own_slice_cap_wf s dq :
-  own_slice_cap s dq -∗ ⌜0 ≤ sint.Z s.(slice.len_f) ≤ sint.Z s.(slice.cap_f)⌝.
+  own_slice_cap s dq -∗ ⌜0 ≤ sint.Z s.(slice.len) ≤ sint.Z s.(slice.cap)⌝.
 Proof.
   unseal. iIntros "[% Hcap]".
   word.
@@ -240,13 +246,13 @@ Qed.
 (* NOTE: only for backwards compatibility; non-primed version is more precise
 about signed length *)
 Lemma own_slice_cap_wf' s dq :
-  own_slice_cap s dq -∗ ⌜uint.Z s.(slice.len_f) ≤ uint.Z s.(slice.cap_f)⌝.
+  own_slice_cap s dq -∗ ⌜uint.Z s.(slice.len) ≤ uint.Z s.(slice.cap)⌝.
 Proof.
   iIntros "H". iDestruct (own_slice_cap_wf with "H") as "%". word.
 Qed.
 
 Lemma own_slice_wf s dq vs :
-  s ↦*{dq} vs -∗ ⌜0 ≤ sint.Z s.(slice.len_f) ≤ sint.Z s.(slice.cap_f)⌝.
+  s ↦*{dq} vs -∗ ⌜0 ≤ sint.Z s.(slice.len) ≤ sint.Z s.(slice.cap)⌝.
 Proof.
   unseal.
   iIntros "[? %]". naive_solver.
@@ -254,7 +260,7 @@ Qed.
 (* NOTE: only for backwards compatibility; non-primed version is more precise
 about signed length *)
 Lemma own_slice_wf' s dq vs :
-  s ↦*{dq} vs -∗ ⌜uint.Z s.(slice.len_f) ≤ uint.Z s.(slice.cap_f)⌝.
+  s ↦*{dq} vs -∗ ⌜uint.Z s.(slice.len) ≤ uint.Z s.(slice.cap)⌝.
 Proof.
   iIntros "H". iDestruct (own_slice_wf with "H") as "%". word.
 Qed.
@@ -268,12 +274,12 @@ Proof.
 Qed.
 
 Lemma slice_to_full_slice s n m :
-  slice.slice_f s t n m = slice.full_slice_f s t n m (slice.cap_f s).
+  slice.slice_f s t n m = slice.full_slice_f s t n m (slice.cap s).
 Proof. reflexivity. Qed.
 
 (* introduce a slice.slice_f for lemmas that require it *)
 Lemma slice_slice_trivial s :
-  s = slice.slice_f s t (W64 0) (slice.len_f s).
+  s = slice.slice_f s t (W64 0) (slice.len s).
 Proof.
   destruct s; simpl.
   rewrite /slice.slice_f /=.
@@ -284,13 +290,13 @@ Qed.
 (* a variant of [slice_slice_trivial] that's easier to use with [iDestruct] and
 more discoverable with Search. *)
 Lemma own_slice_trivial_slice_f s dq (vs: list V) :
-  own_slice s dq vs ⊣⊢ own_slice (slice.slice_f s t (W64 0) (slice.len_f s)) dq vs.
+  own_slice s dq vs ⊣⊢ own_slice (slice.slice_f s t (W64 0) (slice.len s)) dq vs.
 Proof.
   rewrite -slice_slice_trivial //.
 Qed.
 
 Lemma own_slice_trivial_slice_f_2 s dq (vs: list V) :
-  own_slice (slice.slice_f s t (W64 0) (slice.len_f s)) dq vs ⊢ own_slice s dq vs.
+  own_slice (slice.slice_f s t (W64 0) (slice.len s)) dq vs ⊢ own_slice s dq vs.
 Proof.
   rewrite -own_slice_trivial_slice_f //.
 Qed.
@@ -339,14 +345,14 @@ Global Arguments own_slice_cap {_ _ _ _ _} (V) {_ _ _} (s).
 Section wps.
 Context `{hG: heapGS Σ, !ffi_semantics _ _}.
 Lemma wp_slice_len stk E (s : slice.t) (Φ : val -> iProp Σ) :
-    Φ #(s.(slice.len_f)) -∗ WP slice.len (#s) @ stk; E {{ v, Φ v }}.
+    Φ #(s.(slice.len)) -∗ WP slice.len (#s) @ stk; E {{ v, Φ v }}.
 Proof.
   rewrite to_val_unseal. iIntros "HΦ".
   wp_call. rewrite to_val_unseal. iApply "HΦ".
 Qed.
 
 Lemma wp_slice_cap stk E (s : slice.t) (Φ : val -> iProp Σ) :
-    Φ #(s.(slice.cap_f)) -∗ WP slice.cap (#s) @ stk; E {{ v, Φ v }}.
+    Φ #(s.(slice.cap)) -∗ WP slice.cap (#s) @ stk; E {{ v, Φ v }}.
 Proof.
   rewrite to_val_unseal. iIntros "HΦ".
   wp_call. rewrite to_val_unseal. iApply "HΦ".
@@ -394,7 +400,7 @@ Lemma wp_slice_make3 stk E (len cap : w64) :
   {{{ sl, RET #sl;
       sl ↦* (replicate (sint.nat len) (default_val V)) ∗
       own_slice_cap V sl (DfracOwn 1) ∗
-      ⌜ sl.(slice.cap_f) = cap ⌝
+      ⌜ sl.(slice.cap) = cap ⌝
   }}}.
 Proof.
   iIntros (? Φ) "_ HΦ".
@@ -492,7 +498,7 @@ Proof.
 Qed.
 
 Global Instance pure_slice_ptr (s : slice.t) :
-  PureWp True (slice.ptr (#s)) #(slice.ptr_f s).
+  PureWp True (slice.ptr (#s)) #(slice.ptr s).
 Proof.
   rewrite to_val_unseal.
   iIntros (?????) "HΦ".
@@ -501,7 +507,7 @@ Proof.
 Qed.
 
 Global Instance pure_slice_len (s : slice.t) :
-  PureWp True (slice.len (#s)) #(slice.len_f s).
+  PureWp True (slice.len (#s)) #(slice.len s).
 Proof.
   rewrite to_val_unseal.
   iIntros (?????) "HΦ".
@@ -509,7 +515,7 @@ Proof.
 Qed.
 
 Global Instance pure_slice_cap (s : slice.t) :
-  PureWp True (slice.cap (#s)) #(slice.cap_f s).
+  PureWp True (slice.cap (#s)) #(slice.cap s).
 Proof.
   rewrite to_val_unseal.
   iIntros (?????) "HΦ".
@@ -517,7 +523,7 @@ Proof.
 Qed.
 
 Global Instance pure_elem_ref s (i : w64) :
-  PureWp (0 ≤ sint.Z i < sint.Z s.(slice.len_f)) (slice.elem_ref t #s #i)
+  PureWp (0 ≤ sint.Z i < sint.Z s.(slice.len)) (slice.elem_ref t #s #i)
     #(slice.elem_ref_f s t i).
 Proof.
   iIntros (?????) "HΦ".
@@ -528,8 +534,8 @@ Proof.
 Qed.
 
 Global Instance pure_slice_slice s (n m : w64) :
-  PureWp (0 ≤ sint.Z n ≤ sint.Z m ≤ sint.Z (slice.cap_f s) ∧
-          0 ≤ sint.Z (slice.len_f s) ≤ sint.Z (slice.cap_f s)) (slice.slice t #s #n #m)
+  PureWp (0 ≤ sint.Z n ≤ sint.Z m ≤ sint.Z (slice.cap s) ∧
+          0 ≤ sint.Z (slice.len s) ≤ sint.Z (slice.cap s)) (slice.slice t #s #n #m)
     #(slice.slice_f s t n m).
 Proof.
   iIntros (?????) "HΦ".
@@ -552,7 +558,7 @@ Qed.
 
 Global Instance pure_full_slice s (n m c : w64) :
   PureWp (0 ≤ sint.Z n ≤ sint.Z m ≤ sint.Z c ∧
-          0 ≤ sint.Z c ≤ sint.Z (slice.cap_f s)) (slice.full_slice t #s #n #m #c)
+          0 ≤ sint.Z c ≤ sint.Z (slice.cap s)) (slice.full_slice t #s #n #m #c)
     #(slice.full_slice_f s t n m c).
 Proof.
   iIntros (?????) "HΦ".
@@ -581,8 +587,8 @@ TODO: if PureWp instances had their pure side conditions dispatched with [word]
 this lemma would be pretty much unnecessary.
 *)
 Lemma wp_slice_slice_pure s (n m: w64) :
-  {{{ ⌜0 ≤ sint.Z n ≤ sint.Z m ≤ sint.Z s.(slice.cap_f) ∧
-        0 ≤ sint.Z s.(slice.len_f) ≤ sint.Z s.(slice.cap_f)⌝ }}}
+  {{{ ⌜0 ≤ sint.Z n ≤ sint.Z m ≤ sint.Z s.(slice.cap) ∧
+        0 ≤ sint.Z s.(slice.len) ≤ sint.Z s.(slice.cap)⌝ }}}
     slice.slice t #s #n #m
   {{{ RET #(slice.slice_f s t n m); True }}}.
 Proof.
@@ -640,10 +646,10 @@ Proof.
 Qed.
 
 Lemma own_slice_split_all k s dq (vs: list V) :
-  0 ≤ sint.Z k ≤ sint.Z s.(slice.len_f) →
+  0 ≤ sint.Z k ≤ sint.Z s.(slice.len) →
   s ↦*{dq} vs ⊣⊢
   slice.slice_f s t (W64 0) k ↦*{dq} take (sint.nat k) vs ∗
-  slice.slice_f s t k s.(slice.len_f) ↦*{dq} drop (sint.nat k)%nat vs.
+  slice.slice_f s t k s.(slice.len) ↦*{dq} drop (sint.nat k)%nat vs.
 Proof.
   intros Hle.
   rewrite {1}(own_slice_trivial_slice_f s).
@@ -655,14 +661,14 @@ Qed.
 
 (* [own_slice_cap] only depends on where the end of the slice is *)
 Lemma own_slice_cap_same_end s s' dq :
-  slice.ptr_f s +ₗ[t] sint.Z (slice.len_f s) = slice.ptr_f s' +ₗ[t] sint.Z (slice.len_f s') →
-  sint.Z (slice.cap_f s) - sint.Z (slice.len_f s) = sint.Z (slice.cap_f s') - sint.Z (slice.len_f s') →
-  0 ≤ sint.Z (slice.len_f s) ∧ 0 ≤ sint.Z (slice.len_f s') →
+  slice.ptr s +ₗ[t] sint.Z (slice.len s) = slice.ptr s' +ₗ[t] sint.Z (slice.len s') →
+  sint.Z (slice.cap s) - sint.Z (slice.len s) = sint.Z (slice.cap s') - sint.Z (slice.len s') →
+  0 ≤ sint.Z (slice.len s) ∧ 0 ≤ sint.Z (slice.len s') →
   own_slice_cap V s dq ⊣⊢ own_slice_cap V s' dq.
 Proof.
   intros Hend Hcap Hwf.
   rewrite own_slice_cap_unseal /own_slice_cap_def.
-  assert (word.sub (slice.cap_f s) (slice.len_f s) = word.sub (slice.cap_f s') (slice.len_f s'))
+  assert (word.sub (slice.cap s) (slice.len s) = word.sub (slice.cap s') (slice.len s'))
     as Hdiff by word.
   rewrite -Hdiff.
   rewrite -!Hend.
@@ -671,7 +677,7 @@ Proof.
 Qed.
 
 Lemma own_slice_cap_slice_f_change_first s n n' m dq :
-  sint.Z m ≤ sint.Z s.(slice.cap_f) ∧
+  sint.Z m ≤ sint.Z s.(slice.cap) ∧
   0 ≤ sint.Z n ≤ sint.Z m ∧ 0≤ sint.Z n' ≤ sint.Z m →
   own_slice_cap V (slice.slice_f s t n m) dq ⊣⊢ own_slice_cap V (slice.slice_f s t n' m) dq.
 Proof.
@@ -684,8 +690,8 @@ Proof.
 Qed.
 
 Lemma own_slice_cap_slice_f s n dq :
-  0 ≤ sint.Z n ≤ sint.Z (slice.len_f s) ≤ sint.Z (slice.cap_f s) →
-  own_slice_cap V s dq ⊣⊢ own_slice_cap V (slice.slice_f s t n s.(slice.len_f)) dq.
+  0 ≤ sint.Z n ≤ sint.Z (slice.len s) ≤ sint.Z (slice.cap s) →
+  own_slice_cap V s dq ⊣⊢ own_slice_cap V (slice.slice_f s t n s.(slice.len)) dq.
 Proof.
   intros Hwf.
   apply own_slice_cap_same_end; simpl.
@@ -700,13 +706,13 @@ Qed.
 This is not the only choice; see [own_slice_f_cap] for a variation that uses
 capacity. *)
 Lemma own_slice_f (n m: w64) s dq (vs: list V) :
-  0 ≤ sint.Z n ≤ sint.Z m ≤ sint.Z s.(slice.len_f) →
+  0 ≤ sint.Z n ≤ sint.Z m ≤ sint.Z s.(slice.len) →
   s ↦*{dq} vs
   ⊣⊢
   (slice.slice_f s t (W64 0) n) ↦*{dq} (take (sint.nat n) vs) ∗
   (slice.slice_f s t n m) ↦*{dq} (subslice (sint.nat n) (sint.nat m) vs) ∗
   (* after the sliced part *)
-  (slice.slice_f s t m (slice.len_f s)) ↦*{dq} (drop (sint.nat m) vs).
+  (slice.slice_f s t m (slice.len s)) ↦*{dq} (drop (sint.nat m) vs).
 Proof.
   intros. rewrite /subslice.
 
@@ -720,8 +726,8 @@ Proof.
 Qed.
 
 Lemma own_slice_slice_absorb_capacity s (vs: list V) (n m: w64) :
-  0 ≤ sint.Z n ≤ sint.Z m ≤ sint.Z s.(slice.len_f) →
-  slice.slice_f s t m (slice.len_f s) ↦* vs ∗
+  0 ≤ sint.Z n ≤ sint.Z m ≤ sint.Z s.(slice.len) →
+  slice.slice_f s t m (slice.len s) ↦* vs ∗
   own_slice_cap V s (DfracOwn 1) ⊢
   own_slice_cap V (slice.slice_f s t n m) (DfracOwn 1).
 Proof.
@@ -741,7 +747,7 @@ Proof.
   iSplit; [ word | ].
   rewrite Z.mul_0_r loc_add_0 !word.sub_0_r.
   iExists (vs ++ vs').
-  iApply (own_slice_split s.(slice.len_f)).
+  iApply (own_slice_split s.(slice.len)).
   { word. }
   rewrite -> take_app_le, take_ge by (move: Hlen Hlen'; word).
   iFrame "Hvs".
@@ -750,11 +756,11 @@ Proof.
 Qed.
 
 (* divide ownership of [s ↦* vs ∗ own_slice_cap V s] around a slice [slice_f s t
-n m], moving ownership between m and [slice.len_f s] into the capacity of the
+n m], moving ownership between m and [slice.len s] into the capacity of the
 slice *)
 (* TODO: could generalize to ⊣⊢. just need to generalize some deps. *)
 Lemma own_slice_f_cap (n m: w64) s (vs: list V) :
-  0 ≤ sint.Z n ≤ sint.Z m ≤ sint.Z s.(slice.len_f) →
+  0 ≤ sint.Z n ≤ sint.Z m ≤ sint.Z s.(slice.len) →
   s ↦* vs ∗ own_slice_cap V s (DfracOwn 1)
   ⊢
   (slice.slice_f s t (W64 0) n) ↦* (take (sint.nat n) vs) ∗
@@ -776,14 +782,14 @@ TODO: try to avoid using this and use the canonical pure WP for slice.slice (plu
 instead
 *)
 Lemma wp_slice_slice s dq (vs: list V) (n m : w64) :
-  {{{ s ↦*{dq} vs ∗ ⌜0 ≤ sint.Z n ≤ sint.Z m ≤ sint.Z s.(slice.len_f)⌝ }}}
+  {{{ s ↦*{dq} vs ∗ ⌜0 ≤ sint.Z n ≤ sint.Z m ≤ sint.Z s.(slice.len)⌝ }}}
     slice.slice t #s #n #m
   {{{ RET #(slice.slice_f s t n m);
       (* before the sliced part *)
       (slice.slice_f s t (W64 0) n) ↦*{dq} (take (sint.nat n) vs) ∗
       (slice.slice_f s t n m) ↦*{dq} (subslice (sint.nat n) (sint.nat m) vs) ∗
       (* after the sliced part *)
-      (slice.slice_f s t m (slice.len_f s)) ↦*{dq} (drop (sint.nat m) vs)
+      (slice.slice_f s t m (slice.len s)) ↦*{dq} (drop (sint.nat m) vs)
   }}}.
 Proof.
   wp_start as "[Hs %]".
@@ -802,7 +808,7 @@ instead
 *)
 Lemma wp_slice_slice_with_cap s (vs: list V) (n m : w64) :
   {{{ s ↦* vs ∗ own_slice_cap V s (DfracOwn 1) ∗
-            ⌜0 ≤ sint.Z n ≤ sint.Z m ≤ sint.Z s.(slice.len_f)⌝ }}}
+            ⌜0 ≤ sint.Z n ≤ sint.Z m ≤ sint.Z s.(slice.len)⌝ }}}
     slice.slice t #s #n #m
   {{{ RET #(slice.slice_f s t n m);
       (* before the sliced part *)
@@ -826,7 +832,7 @@ Qed.
 moves elements from the hidden capacity of s into its actual contents. *)
 Lemma own_slice_slice_into_capacity (n m: w64) s (vs: list V) :
   s ↦* vs ∗ own_slice_cap V s (DfracOwn 1) ∗
-      ⌜0 ≤ sint.Z n ∧ sint.Z n ≤ sint.Z s.(slice.len_f) ≤ sint.Z m ≤ sint.Z s.(slice.cap_f)⌝ ⊢
+      ⌜0 ≤ sint.Z n ∧ sint.Z n ≤ sint.Z s.(slice.len) ≤ sint.Z m ≤ sint.Z s.(slice.cap)⌝ ⊢
   ∃ (vs': list V),
   (slice.slice_f s t (W64 0) n) ↦* (take (sint.nat n) vs) ∗
       (slice.slice_f s t n m) ↦* (drop (sint.nat n) vs ++ vs') ∗
@@ -839,17 +845,17 @@ Proof.
   iDestruct "Hcap" as "[_ [%vs' Hcap]]".
   iDestruct (own_slice_len with "Hcap") as %Hlen'.
   simpl in Hlen'.
-  iExists (take (sint.nat m - sint.nat s.(slice.len_f))%nat vs').
+  iExists (take (sint.nat m - sint.nat s.(slice.len))%nat vs').
   iDestruct (own_slice_split_all n with "Hs") as "[Hs1 Hs2]";
     [ word | ].
-  iDestruct (own_slice_split_all (word.sub m s.(slice.len_f)) with "Hcap") as "[Hvs' Hcap']".
+  iDestruct (own_slice_split_all (word.sub m s.(slice.len)) with "Hcap") as "[Hvs' Hcap']".
   { simpl. word. }
   simpl.
   iSplitL "Hs1".
   { iFrame. }
   iSplitL "Hs2 Hvs'".
   {
-    iApply (own_slice_split s.(slice.len_f)).
+    iApply (own_slice_split s.(slice.len)).
     { word. }
     iSplitL "Hs2".
     { iExactEq "Hs2".
@@ -865,9 +871,9 @@ Proof.
     rewrite drop_drop.
     rewrite -> drop_ge by len.
     rewrite app_nil_l.
-    replace (sint.nat (word.sub m (slice.len_f s))) with
-      (sint.nat m - sint.nat (slice.len_f s))%nat by word.
-    set (k := (sint.nat m - sint.nat (slice.len_f s))%nat).
+    replace (sint.nat (word.sub m (slice.len s))) with
+      (sint.nat m - sint.nat (slice.len s))%nat by word.
+    set (k := (sint.nat m - sint.nat (slice.len s))%nat).
 
     rewrite own_slice_unseal /own_slice_def /=.
     iDestruct "Hvs'" as "[Hvs' %Hwf']".
@@ -882,7 +888,7 @@ Proof.
   }
   iSplit.
   { iPureIntro; move: Hlen'; len. }
-  iExists (drop (sint.nat (word.sub m (slice.len_f s))) vs').
+  iExists (drop (sint.nat (word.sub m (slice.len s))) vs').
   rewrite /slice.slice_f /=.
   rewrite !loc_add_assoc -!Z.mul_add_distr_l.
   iExactEq "Hcap'".
@@ -890,31 +896,31 @@ Proof.
 
   (* FIXME: automate these simplifications that were helpful to see the proof *)
   (*
-  replace (word.sub (word.sub (slice.cap_f s) (slice.len_f s)) (word.sub m (slice.len_f s))) with
-    (word.sub s.(slice.cap_f) m) by word.
-  replace (word.sub (word.sub (slice.cap_f s) n) (word.sub m n))
-            with (word.sub s.(slice.cap_f) m) by word.
+  replace (word.sub (word.sub (slice.cap s) (slice.len s)) (word.sub m (slice.len s))) with
+    (word.sub s.(slice.cap) m) by word.
+  replace (word.sub (word.sub (slice.cap s) n) (word.sub m n))
+            with (word.sub s.(slice.cap) m) by word.
   replace (uint.Z n + uint.Z (word.sub m n)) with
     (uint.Z m) by word.
-  replace (uint.Z (slice.len_f s) + uint.Z (word.sub m (slice.len_f s))) with
+  replace (uint.Z (slice.len s) + uint.Z (word.sub m (slice.len s))) with
     (uint.Z m) by word.
 
-  iDestruct (own_slice_split (word.sub s.(slice.cap_f) s.(slice.len_f)) with "Hcap'") as "[_ Hcap]".
+  iDestruct (own_slice_split (word.sub s.(slice.cap) s.(slice.len)) with "Hcap'") as "[_ Hcap]".
   { word. }
   rewrite /slice.slice_f /=.
   rewrite !loc_add_assoc -!Z.mul_add_distr_l.
-  replace (uint.nat (word.sub m s.(slice.len_f))) with (uint.nat m - uint.nat s.(slice.len_f))%nat by word.
-  replace (uint.nat (word.sub s.(slice.cap_f) s.(slice.len_f))) with (uint.nat s.(slice.cap_f) - uint.nat s.(slice.len_f))%nat by word.
+  replace (uint.nat (word.sub m s.(slice.len))) with (uint.nat m - uint.nat s.(slice.len))%nat by word.
+  replace (uint.nat (word.sub s.(slice.cap) s.(slice.len))) with (uint.nat s.(slice.cap) - uint.nat s.(slice.len))%nat by word.
   replace (uint.Z n + uint.Z (word.sub m n)) with (uint.Z m) by word.
   rewrite drop_drop.
-  replace (uint.nat m - uint.nat (slice.len_f s) +
-     (uint.nat (slice.cap_f s) -
-        uint.nat (slice.len_f s) -
+  replace (uint.nat m - uint.nat (slice.len s) +
+     (uint.nat (slice.cap s) -
+        uint.nat (slice.len s) -
         (uint.nat m -
-           uint.nat (slice.len_f s))))%nat with
-    (uint.nat s.(slice.cap_f) - uint.nat s.(slice.len_f))%nat by word.
-  iExists (drop (uint.nat (slice.cap_f s) -
-                   uint.nat (slice.len_f s))
+           uint.nat (slice.len s))))%nat with
+    (uint.nat s.(slice.cap) - uint.nat s.(slice.len))%nat by word.
+  iExists (drop (uint.nat (slice.cap s) -
+                   uint.nat (slice.len s))
              vs').
 *)
 Qed.
@@ -1163,7 +1169,7 @@ Proof.
       "Hs1" ∷ s ↦* (take (sint.nat i) vs' ++ drop (sint.nat i) vs) ∗
       "Hs2" ∷ s2 ↦*{dq} vs' ∗
       "i" ∷ i_ptr ↦ i ∗
-      "%" ∷ ⌜0 ≤ sint.Z i ≤ Z.min (sint.Z s.(slice.len_f)) (sint.Z s2.(slice.len_f))⌝
+      "%" ∷ ⌜0 ≤ sint.Z i ≤ Z.min (sint.Z s.(slice.len)) (sint.Z s2.(slice.len))⌝
     )%I with "[Hs1 Hs2 i]" as "IH".
   { iFrame. simpl. word. }
   wp_for "IH".
@@ -1199,7 +1205,7 @@ Proof.
     2: { inv 1. }
     rewrite decide_True //.
     wp_auto.
-    assert (i = slice.len_f s2) by word; subst i.
+    assert (i = slice.len s2) by word; subst i.
     iApply "HΦ".
     iSplit; [ word | ].
     iFrame "Hs2".
@@ -1210,7 +1216,7 @@ Proof.
     2: { inv 1. }
     rewrite decide_True //.
     wp_auto.
-    assert (i = slice.len_f s) by word; subst i.
+    assert (i = slice.len s) by word; subst i.
     iApply "HΦ".
     iSplit; [ word | ].
     iFrame "Hs2".
@@ -1229,8 +1235,8 @@ Qed.
 
 Lemma own_slice_zero_size (s: slice.t) (vs: list V) dq :
   go_type_size t = 0%nat →
-  length vs = uint.nat (slice.len_f s) →
-  0 ≤ sint.Z s.(slice.len_f) ≤ sint.Z s.(slice.cap_f) →
+  length vs = uint.nat (slice.len s) →
+  0 ≤ sint.Z s.(slice.len) ≤ sint.Z s.(slice.cap) →
   ⊢ s ↦*{dq} vs.
 Proof using IntoValTyped0.
   intros Hz Hlen Hwf.
@@ -1243,13 +1249,13 @@ Qed.
 
 Lemma own_slice_cap_zero_size (s: slice.t) :
   go_type_size t = 0%nat →
-  0 ≤ sint.Z s.(slice.len_f) ≤ sint.Z s.(slice.cap_f) →
+  0 ≤ sint.Z s.(slice.len) ≤ sint.Z s.(slice.cap) →
   ⊢ own_slice_cap V s (DfracOwn 1).
 Proof using IntoValTyped0.
   intros Hz Hwf.
   rewrite own_slice_cap_unseal /own_slice_cap_def.
   iSplit; [ word | ].
-  iExists (replicate (sint.nat (word.sub (slice.cap_f s) (slice.len_f s))) (default_val V)).
+  iExists (replicate (sint.nat (word.sub (slice.cap s) (slice.len s))) (default_val V)).
   iApply own_slice_zero_size; simpl; auto; len.
 Qed.
 
@@ -1297,7 +1303,7 @@ Proof.
     iClear "Hs". (* empty *)
     iDestruct (own_slice_len with "Hs_new") as %Hlen.
     simpl in Hlen; autorewrite with len in Hlen.
-    assert (length vs'' = sint.nat s2.(slice.len_f)) by (move: Hlen; word).
+    assert (length vs'' = sint.nat s2.(slice.len)) by (move: Hlen; word).
     wp_apply (wp_slice_slice_with_cap with "[$Hs_new $Hcap]").
     { iPureIntro; simpl; by len. }
     iIntros "(Hs_new1 & Hs_new2 & Hs_new_cap)".
@@ -1312,7 +1318,7 @@ Proof.
     iApply "HΦ".
     iFrame "Hs2".
     iSplitL "Hs_new1 Hs_new2".
-    { iDestruct (own_slice_combine s.(slice.len_f) with "Hs_new1 Hs_new2") as "Hs_new".
+    { iDestruct (own_slice_combine s.(slice.len) with "Hs_new1 Hs_new2") as "Hs_new".
       { len. }
       rewrite -> !take_app_le, !take_ge by word.
       iFrame "Hs_new".
@@ -1326,7 +1332,7 @@ Proof.
     iDestruct (own_slice_wf with "Hnew") as %Hsl_wf.
     iDestruct (own_slice_len with "Hnew") as %Hsl_len.
     autorewrite with len in Hsl_len.
-    assert (word.add (slice.len_f s) (slice.len_f s2) = slice.len_f sl) as Hsl_len'.
+    assert (word.add (slice.len s) (slice.len s2) = slice.len sl) as Hsl_len'.
     { apply word.unsigned_inj.
       move: Hsl_len; word. }
     wp_pures.
